viper-total-heaps/TotalConsistencyInst.thy
@@ -8,7 +8,13 @@ subsection \<open>Internal Consistency Wellfoundness\<close>
 lemma wf_total_consistency_internal: "wf_total_consistency ctxt consistent_internal_total_full consistent_internal_total"
   unfolding wf_total_consistency_def
   apply (intro conjI)
-  sorry
+      apply (rule intcons_mono_prop_downward)
+     apply (simp add: intcons_empty is_empty_total_full_def)
+  using intcons_preserved_by_red_stmt
+    apply blast
+   apply (simp add: intcons_preserved_by_update_store)
+  using consistent_internal_total_full_def
+  by blast
 
 
 end
