viper-total-heaps/TotalSemantics.thy
@@ -536,7 +536,7 @@ these properties.\<close>
 definition wf_total_consistency
   where "wf_total_consistency ctxt R Rt \<equiv>
                mono_prop_downward R \<and>
-               (\<forall>\<omega>. is_empty_total_full \<omega> \<longrightarrow> R \<omega>) \<and>
+               (\<forall>\<omega>. is_empty_total_full \<omega> \<longrightarrow> Rt (get_total_full \<omega>)) \<and>
                (\<forall>\<omega> \<omega>' \<Lambda> stmt. R \<omega> \<longrightarrow> red_stmt_total ctxt R \<Lambda> stmt \<omega> (RNormal \<omega>') \<longrightarrow> R \<omega>') \<and>
                \<comment>\<open>The following statement ensures that states in the body of a scope preserve consistency.\<close>
                (\<forall>\<omega> v. R \<omega> \<longrightarrow> R (shift_and_add_state_total \<omega> v)) \<and>
