viper-total-heaps/TotalSemanticsHelper.thy
@@ -65,6 +65,10 @@ lemmas red_inhale_elims =
 
 subsubsection \<open>Exhale\<close>
 
+inductive_cases ExhAcc_case: "red_exhale ctxt R \<omega>0 (Atomic (Acc e_r f perm)) \<omega> (RNormal \<omega>')"
+inductive_cases ExhAccPred_case: "red_exhale ctxt R \<omega>0 (Atomic (AccPredicate pid e_args perm)) \<omega> (RNormal \<omega>')"
+inductive_cases ExhAccPredWildcard_case: "red_exhale ctxt R \<omega>0 (Atomic (AccPredicate pid e_args Wildcard)) \<omega> (RNormal \<omega>')"
+inductive_cases ExhImp_case: "red_exhale ctxt R \<omega>0 (Imp e A) \<omega> (RNormal \<omega>')"
 inductive_cases ExhStar_case: "red_exhale ctxt R \<omega>0 (A && B) m_pm res"
 
 lemma ExhPure_case:
